{
 "cells": [
  {
   "cell_type": "markdown",
   "metadata": {},
   "source": [
    "$$\n",
    "\\begin{align*}\n",
    "x(t) &= [\\sqrt{D^2 - z^2}]\\cos(t) + x_1\\\\\n",
    "y(t) &= [\\sqrt{D^2 - z^2}]\\sin(t) + y_1\\\\\n",
    "\n",
    "r(t) &= \\sqrt{[D^2 - z^2]\\cos^2(t) + x_1^2 + x_1[\\sqrt{D^2 - z^2}]\\cos(t) + [D^2 - z^2]\\sin^2(t) + y_1^2 + y_1[\\sqrt{D^2 - z^2}]\\sin(t) + z^2}\\\\\n",
    "&= \\sqrt{[D^2 - z^2] + x_1^2 + y_1^2 + z^2 + [\\sqrt{D^2 - z^2}](x_1\\cos(t)+y_1\\sin(t))}\\\\\n",
    "&= \\sqrt{D^2 + x_1^2 + y_1^2 + [\\sqrt{D^2 - z^2}](x_1\\cos(t)+y_1\\sin(t))}\\\\\n",
    "\n",
    "\\frac{dx}{dt} &= -[\\sqrt{D^2 - z^2}]\\sin(t)\\\\\n",
    "\\frac{dy}{dt} &= [\\sqrt{D^2 - z^2}]\\cos(t)\\\\\n",
    "\n",
    "{\\begin{bmatrix} \\frac{dx}{dt} \\end{bmatrix}}^2 &= (D^2 - z^2)\\sin^2(t)\\\\\n",
    "{\\begin{bmatrix} \\frac{dy}{dt} \\end{bmatrix}}^2 &= (D^2 - z^2)\\cos^2(t)\\\\\n",
    "\n",
    "{\\begin{bmatrix} \\frac{dx}{dt} \\end{bmatrix}}^2 + {\\begin{bmatrix} \\frac{dy}{dt} \\end{bmatrix}}^2 &= (D^2 - z^2)\\sin^2(t) + (D^2 - z^2)\\cos^2(t)\\\\\n",
    "{\\begin{bmatrix} \\frac{dx}{dt} \\end{bmatrix}}^2 + {\\begin{bmatrix} \\frac{dy}{dt} \\end{bmatrix}}^2 &= (D^2 - z^2)\\sin^2(t) + (D^2 - z^2)\\cos^2(t)\\\\\n",
    "\n",
    "\\text{If we have a density $\\rho$, such that } \\rho &= \\rho(r),\\\\\n",
    "\\text{we can say } \\rho(r) &= \\rho(x,y,z) = \\rho(\\sqrt{x^2 + y^2 + z^2})\\\\\n",
    "\\text{The mass around the circle } &= \\int_0^{2\\pi} \\rho(x(t),y(t),z(t))\\sqrt{\\dot{x}(t)^2 + \\dot{y}(t)^2 + \\dot{z}(t)^2} \\; dt\\\\\n",
    "\\text{The mass around a sphere of radius D } &= \\int_{-D}^{D} \\frac{D}{\\sqrt{D^2 - z^2}} \\int_0^{2\\pi} \\rho(x(t),y(t),z)\\sqrt{\\dot{x}(t)^2 + \\dot{y}(t)^2} \\; dt \\: dz \\\\\n",
    "&= \\int_{-D}^{D} \\frac{D}{\\sqrt{D^2 - z^2}} \\int_0^{2\\pi} \\rho(\\sqrt{(D^2 - z^2)\\cos^2(t) + (D^2 - z^2)\\sin^2(t) + z^2})\\sqrt{\\dot{x}(t)^2 + \\dot{y}(t)^2} \\; dt \\: dz \\\\\n",
    "\n",
    "&= \\int_{-D}^{D} \\frac{D}{\\sqrt{D^2 - z^2}} \\int_0^{2\\pi} \\rho(\\sqrt{D^2 - z^2 + z^2})\\sqrt{\\dot{x}(t)^2 + \\dot{y}(t)^2} \\; dt \\: dz \\\\\n",
    "\n",
    "&= \\int_{-D}^{D} \\frac{D}{\\sqrt{D^2 - z^2}} \\int_0^{2\\pi} \\rho(D)\\sqrt{\\dot{x}(t)^2 + \\dot{y}(t)^2} \\; dt \\: dz \\\\\n",
    "\\end{align*}\n",
    "$$"
   ]
  },
  {
   "cell_type": "markdown",
   "metadata": {},
   "source": []
  }
 ],
 "metadata": {
  "language_info": {
   "name": "python"
  },
  "orig_nbformat": 4
 },
 "nbformat": 4,
 "nbformat_minor": 2
}
